add a F# hash checker, move common OCaml/F# hash checker parts to F*

src/3d/hashchk/3d/HashingOptions.fs
@@ -1,0 +1,193 @@
+#light "off"
+module HashingOptions
+open Prims
+open FStar_Pervasives
+type check_hashes_t =
+| WeakHashes
+| StrongHashes
+| InplaceHashes
+
+
+let uu___is_WeakHashes : check_hashes_t  ->  Prims.bool = (fun ( projectee  :  check_hashes_t ) -> (match (projectee) with
+| WeakHashes -> begin
+true
+end
+| uu___ -> begin
+false
+end))
+
+
+let uu___is_StrongHashes : check_hashes_t  ->  Prims.bool = (fun ( projectee  :  check_hashes_t ) -> (match (projectee) with
+| StrongHashes -> begin
+true
+end
+| uu___ -> begin
+false
+end))
+
+
+let uu___is_InplaceHashes : check_hashes_t  ->  Prims.bool = (fun ( projectee  :  check_hashes_t ) -> (match (projectee) with
+| InplaceHashes -> begin
+true
+end
+| uu___ -> begin
+false
+end))
+
+
+let is_weak : check_hashes_t  ->  Prims.bool = (fun ( uu___  :  check_hashes_t ) -> (match (uu___) with
+| WeakHashes -> begin
+true
+end
+| InplaceHashes -> begin
+true
+end
+| uu___1 -> begin
+false
+end))
+
+type micro_step_t =
+| MicroStepVerify
+| MicroStepExtract
+| MicroStepCopyClangFormat
+| MicroStepCopyEverParseH
+| MicroStepEmitConfig
+
+
+let uu___is_MicroStepVerify : micro_step_t  ->  Prims.bool = (fun ( projectee  :  micro_step_t ) -> (match (projectee) with
+| MicroStepVerify -> begin
+true
+end
+| uu___ -> begin
+false
+end))
+
+
+let uu___is_MicroStepExtract : micro_step_t  ->  Prims.bool = (fun ( projectee  :  micro_step_t ) -> (match (projectee) with
+| MicroStepExtract -> begin
+true
+end
+| uu___ -> begin
+false
+end))
+
+
+let uu___is_MicroStepCopyClangFormat : micro_step_t  ->  Prims.bool = (fun ( projectee  :  micro_step_t ) -> (match (projectee) with
+| MicroStepCopyClangFormat -> begin
+true
+end
+| uu___ -> begin
+false
+end))
+
+
+let uu___is_MicroStepCopyEverParseH : micro_step_t  ->  Prims.bool = (fun ( projectee  :  micro_step_t ) -> (match (projectee) with
+| MicroStepCopyEverParseH -> begin
+true
+end
+| uu___ -> begin
+false
+end))
+
+
+let uu___is_MicroStepEmitConfig : micro_step_t  ->  Prims.bool = (fun ( projectee  :  micro_step_t ) -> (match (projectee) with
+| MicroStepEmitConfig -> begin
+true
+end
+| uu___ -> begin
+false
+end))
+
+type makefile_type =
+| MakefileGMake
+| MakefileNMake
+
+
+let uu___is_MakefileGMake : makefile_type  ->  Prims.bool = (fun ( projectee  :  makefile_type ) -> (match (projectee) with
+| MakefileGMake -> begin
+true
+end
+| uu___ -> begin
+false
+end))
+
+
+let uu___is_MakefileNMake : makefile_type  ->  Prims.bool = (fun ( projectee  :  makefile_type ) -> (match (projectee) with
+| MakefileNMake -> begin
+true
+end
+| uu___ -> begin
+false
+end))
+
+type input_stream_binding_t =
+| InputStreamBuffer
+| InputStreamExtern of Prims.string
+| InputStreamStatic of Prims.string
+
+
+let uu___is_InputStreamBuffer : input_stream_binding_t  ->  Prims.bool = (fun ( projectee  :  input_stream_binding_t ) -> (match (projectee) with
+| InputStreamBuffer -> begin
+true
+end
+| uu___ -> begin
+false
+end))
+
+
+let uu___is_InputStreamExtern : input_stream_binding_t  ->  Prims.bool = (fun ( projectee  :  input_stream_binding_t ) -> (match (projectee) with
+| InputStreamExtern (include_file) -> begin
+true
+end
+| uu___ -> begin
+false
+end))
+
+
+let __proj__InputStreamExtern__item__include_file : input_stream_binding_t  ->  Prims.string = (fun ( projectee  :  input_stream_binding_t ) -> (match (projectee) with
+| InputStreamExtern (include_file) -> begin
+include_file
+end))
+
+
+let uu___is_InputStreamStatic : input_stream_binding_t  ->  Prims.bool = (fun ( projectee  :  input_stream_binding_t ) -> (match (projectee) with
+| InputStreamStatic (include_file) -> begin
+true
+end
+| uu___ -> begin
+false
+end))
+
+
+let __proj__InputStreamStatic__item__include_file : input_stream_binding_t  ->  Prims.string = (fun ( projectee  :  input_stream_binding_t ) -> (match (projectee) with
+| InputStreamStatic (include_file) -> begin
+include_file
+end))
+
+
+let string_of_input_stream_binding : input_stream_binding_t  ->  Prims.string = (fun ( uu___  :  input_stream_binding_t ) -> (match (uu___) with
+| InputStreamBuffer -> begin
+"buffer"
+end
+| InputStreamExtern (uu___1) -> begin
+"extern"
+end
+| InputStreamStatic (uu___1) -> begin
+"static"
+end))
+
+
+let input_stream_include : input_stream_binding_t  ->  Prims.string = (fun ( uu___  :  input_stream_binding_t ) -> (match (uu___) with
+| InputStreamBuffer -> begin
+""
+end
+| InputStreamStatic (s) -> begin
+s
+end
+| InputStreamExtern (s) -> begin
+s
+end))
+
+
+
+
