src/3d/hashchk/3d/Version.fs
@@ -1,0 +1,4 @@
+module Version
+let everparse_version = "v2024.08.23"
+let fstar_commit = "8b2041e93d"
+let karamel_commit = "ba951d85"
