src/3d/hashchk/Program.fs
@@ -1,0 +1,136 @@
+﻿// Learn more about F# at http://docs.microsoft.com/dotnet/fsharp
+// See the 'F# Tutorial' project for more help.
+
+module Program
+
+let check_inplace_hashes_f h file_c =
+    let arr = System.IO.File.ReadAllLines(file_c)
+    let len = arr.Length
+    (* Check fails if a bad hash or no hash is found. A
+       good hash alone does not make the check succeed *)
+    let rec aux accu i =
+      if i = len
+      then accu
+      else
+        let r = arr.[i].Trim().Split(':')
+        let j = i + 1
+        if (r.Length <> 2)
+        then aux accu j
+        else if r.[0] <> Hashing_Hash.c_comment_intro
+        then aux accu j
+        else if r.[1] = h
+        then aux (Some true) j
+        else
+          let msg = System.String.Concat("Weak hash check failed in ", file_c)
+          let msg = System.String.Concat(msg, ", expected ")
+          let msg = System.String.Concat(msg, h)
+          let msg = System.String.Concat(msg, ", found ")
+          let msg = System.String.Concat(msg, r.[1])
+          System.Console.WriteLine msg
+          Some false
+     in
+     match aux None 0 with
+     | None ->
+       System.Console.WriteLine (System.String.Concat ("No hash found in ", file_c))
+       false
+     | Some res -> res
+
+let hash_file filename =
+    use h = System.Security.Cryptography.SHA256.Create ()
+    use f = System.IO.File.OpenRead(filename)
+    let a = h.ComputeHash(f)
+    let sp = System.ReadOnlySpan(a, 0, a.Length)
+    Hashing_Op.bytes_to_hex sp
+
+let everparse_version = "2024.08.23"
+
+let everparse_url =
+  let suffix =
+    if System.Runtime.InteropServices.RuntimeInformation.IsOSPlatform(System.Runtime.InteropServices.OSPlatform.Linux)
+    then "Linux_x86_64.tar.gz"
+    else if System.Runtime.InteropServices.RuntimeInformation.IsOSPlatform(System.Runtime.InteropServices.OSPlatform.Windows)
+    then "Windows_NT_x86_64.zip"
+    else failwith "everparse_url: Cannot determine OS platform"
+  in
+  "https://github.com/project-everest/everparse/releases/download/v" ^ everparse_version ^ "/everparse_v" ^ everparse_version ^ "_" ^ suffix
+
+let everparse_filename =
+  let suffix =
+    if System.Runtime.InteropServices.RuntimeInformation.IsOSPlatform(System.Runtime.InteropServices.OSPlatform.Linux)
+    then "tar.gz"
+    else if System.Runtime.InteropServices.RuntimeInformation.IsOSPlatform(System.Runtime.InteropServices.OSPlatform.Windows)
+    then "zip"
+    else failwith "everparse_filename: Cannot determine OS platform"
+  in
+  "everparse." ^ suffix
+
+let everparse_hash =
+  if System.Runtime.InteropServices.RuntimeInformation.IsOSPlatform(System.Runtime.InteropServices.OSPlatform.Linux)
+  then "e731ab039ab9b228afd3393ac39d453697234aed5fe1296ecbf253cb59ce5fcc"
+  else if System.Runtime.InteropServices.RuntimeInformation.IsOSPlatform(System.Runtime.InteropServices.OSPlatform.Windows)
+  then "b71fd70319bf111d21474a4e7d332274ad648181c8c368e2d7287150b940f234"
+  else failwith "everparse_filename: Cannot determine OS platform"
+
+let everparse_unpack () =
+  if System.Runtime.InteropServices.RuntimeInformation.IsOSPlatform(System.Runtime.InteropServices.OSPlatform.Linux) then
+    use f = System.IO.File.OpenRead(everparse_filename)
+    use gz = new System.IO.Compression.GZipStream(f, System.IO.Compression.CompressionMode.Decompress)
+    System.Formats.Tar.TarFile.ExtractToDirectory(gz, ".", false)
+  else if System.Runtime.InteropServices.RuntimeInformation.IsOSPlatform(System.Runtime.InteropServices.OSPlatform.Windows) then
+    System.IO.Compression.ZipFile.ExtractToDirectory(everparse_filename, ".", false)
+  else
+    failwith "everparse_unpack: Cannot determine OS platform"
+
+let everparse_pkg_entrypoint dirname =
+  if System.Runtime.InteropServices.RuntimeInformation.IsOSPlatform(System.Runtime.InteropServices.OSPlatform.Linux) then
+    System.IO.Path.Combine(dirname, "everparse.sh")
+  else if System.Runtime.InteropServices.RuntimeInformation.IsOSPlatform(System.Runtime.InteropServices.OSPlatform.Windows) then
+    System.IO.Path.Combine(dirname, "everparse.cmd")
+  else
+    failwith "everparse_pkg_entrypoint: Cannot determine OS platform"
+
+[<EntryPoint>]
+let main _ =
+  (* Parse command-line options. This action is only accumulating values into globals, without any further action (other than --help and --version, which interrupt the execution.) *)
+  let _ = Options.parse_cmd_line() in
+  (* Special mode: --check_inplace_hashes *)
+  let inplace_hashes = Options.check_inplace_hashes () in
+  if not (List.isEmpty inplace_hashes)
+  then
+    Hashing_Hash.check_inplace_hashes check_inplace_hashes_f inplace_hashes
+    exit 0
+  System.Console.WriteLine "You are trying to call the EverParse/3d inplace hash checker with an unsupported EverParse/3d option. The only supported option is --check_inplace_hash . Do you want to try downloading a full EverParse binary package from GitHub Releases and running it? (y/N)" // please download and use a full EverParse binary package from https://github.com/project-everest/everparse/releases"
+  if System.Console.ReadKey().KeyChar.ToString() <> "y" then
+     exit 1
+  let dirname =
+    let everparse_home = System.Environment.GetEnvironmentVariable("EVERPARSE_HOME")
+    if (everparse_home = null) then
+       System.Console.WriteLine "EVERPARSE_HOME not defined"
+       let dirname = "everparse"
+       if System.IO.Directory.Exists(dirname) then
+         System.Console.WriteLine ("Using existing " ^ dirname ^ " subdirectory")
+       else
+         System.Console.WriteLine (dirname ^ " subdirectory not found")
+         use wc = new System.Net.WebClient ()
+         if System.IO.File.Exists(everparse_filename) then
+           System.Console.WriteLine ("Found binary package " ^ everparse_filename)
+         else
+           System.Console.WriteLine ("Binary package not found. Downloading from " ^ everparse_url)
+           wc.DownloadFile(everparse_url, everparse_filename)
+         let s = hash_file everparse_filename
+         System.Console.WriteLine ("Expected hash: " ^ everparse_hash)
+         System.Console.WriteLine ("Found hash: " ^ s)
+         if s <> everparse_hash then
+           System.Console.WriteLine ("Failed to download EverParse: hash mismatch")
+           exit 1
+         System.Console.WriteLine ("Unpacking " ^ everparse_filename)
+         everparse_unpack ()
+       dirname
+    else
+      System.Console.WriteLine ("Using EverParse from EVERPARSE_HOME = " ^ everparse_home)
+      everparse_home
+  let argv = System.Environment.GetCommandLineArgs()
+  let args = System.ArraySegment(argv, 1, argv.Length - 1)
+  use p = System.Diagnostics.Process.Start(everparse_pkg_entrypoint dirname, args)
+  p.WaitForExit ()
+  p.ExitCode
