src/3d/ocaml/sha/HashingBase.ml
@@ -1,7 +1,38 @@
 type t = Sha256.ctx
 
+let debug_hash = false
+
 let init () = Sha256.init ()
 
-let update h b = Sha256.update_string h (Bytes.to_string b)
-
 let finish h = Bytes.of_string (Sha256.to_bin (Sha256.finalize h))
+
+let char_of_int4 x =
+  assert (0 <= x && x < 16);
+  if x < 10
+  then char_of_int (int_of_char '0' + x)
+  else char_of_int (int_of_char 'a' + x - 10)
+
+let hex_of_char c =
+  let i = int_of_char c in
+  assert (0 <= i && i < 256);
+  char_of_int4 (i / 16), char_of_int4 (i mod 16)
+
+let hex_of_bytes buf =
+  let hex = Bytes.create (Bytes.length buf * 2) in
+  Bytes.iteri (fun idx c ->
+      let hi, lo = hex_of_char c in
+      Bytes.set hex (2 * idx) hi;
+      Bytes.set hex (2 * idx + 1) lo
+    ) buf;
+  Bytes.to_string hex
+
+let update h b =
+  if debug_hash then begin
+      print_endline ("Trying to update with: " ^ hex_of_bytes b);
+  end;
+  Sha256.update_string h (Bytes.to_string b);
+  if debug_hash then begin
+      let h' = Sha256.copy h in
+      let s = finish h' in
+      print_endline ("Update: " ^ hex_of_bytes s)
+  end
