src/3d/Hashing.Hash.fst
@@ -1,0 +1,87 @@
+module Hashing.Hash
+open Hashing.Op
+
+type c_files = {
+    wrapper_h: option string;
+    wrapper_c: option string;
+    h: string;
+    c: string;
+    assertions: option string;
+  }
+
+let hash f opt_c =
+  let h = hash_init () in
+  hash_string h Version.everparse_version;
+  hash_string h Version.fstar_commit;
+  hash_string h Version.karamel_commit;
+  hash_file h f;
+  begin match opt_c with
+  | None -> hash_bool h false
+  | Some c ->
+     hash_bool h true;
+     hash_file_option h c.wrapper_h;
+     hash_file_option h c.wrapper_c;
+     hash_file h c.h;
+     hash_file h c.c;
+     begin match c.assertions with
+     | None ->
+        hash_bool h false
+     | Some assertions ->
+        hash_bool h true;
+        hash_file h assertions
+     end
+  end;
+  hash_finish h
+
+let c_comment_intro = "EverParse checksum hash"
+
+let hash_as_comment file =
+  let h = hash file None in
+  c_comment_intro ^ ":" ^ h
+
+type check_inplace_hashes_t =
+  | AllHashes of c_files
+  | OneHash of string
+
+let check_inplace_hashes_on f file_3d files_c =
+  let h = hash file_3d None in
+  match files_c with
+  | OneHash c_file -> f h c_file
+  | AllHashes files_c ->
+    List.for_all (f h) (
+      files_c.c ::
+      files_c.h ::
+      begin match files_c.wrapper_c with
+      | None -> []
+      | Some w -> [w]
+      end @
+      begin match files_c.wrapper_h with
+      | None -> []
+      | Some w -> [w]
+      end @
+      begin match files_c.assertions with
+      | None -> []
+      | Some assertions -> [assertions]
+      end
+    )
+
+let check_inplace_hash
+     f file_3d_file_c
+  =
+  let eqstr' () : FStar.All.ML (s: string { String.length s == 1 }) =
+    assert_norm (String.length "=" == 1);
+    "="
+  in
+  let eqstr = eqstr' () in
+  match String.split [String.index eqstr 0] file_3d_file_c with
+  | [file_3d; file_c] ->
+     if check_inplace_hashes_on f file_3d (OneHash file_c)
+     then begin
+         FStar.IO.print_string (Printf.sprintf "EverParse check_inplace_hash succeeded on %s\n" file_3d)
+       end else begin
+         FStar.IO.print_string (Printf.sprintf "EverParse check_inplace_hash failed on %s\n" file_3d);
+         FStar.All.exit 255
+       end
+  | _ -> FStar.All.failwith "check_inplace_hash: expected file.3d=file.h"
+
+let check_inplace_hashes f = List.iter (check_inplace_hash f)
