src/3d/Options.fsti
@@ -8,76 +8,76 @@ val compute_options (ignore: list string) : ML string
 
 val parse_cmd_line : unit -> ML (list string)
 
-val get_file_name (mname:string) : ML string
+val file_name (mname:string) : ML string
 
-val get_module_name (file: string) : ML string
+val module_name (file: string) : ML string
 
-val get_output_dir : unit -> ML string
+val output_dir : unit -> ML string
 
 val debug_print_string (s:string) : ML unit
 
-val get_batch : unit -> ML bool
+val batch : unit -> ML bool
 
-val get_clang_format : unit -> ML bool
+val clang_format : unit -> ML bool
 
-val get_clang_format_executable : unit -> ML string
+val clang_format_executable : unit -> ML string
 
-val get_cleanup : unit -> ML bool
+val cleanup : unit -> ML bool
 
-val get_skip_c_makefiles : unit -> ML bool
+val skip_c_makefiles : unit -> ML bool
 
-val get_no_everparse_h : unit -> ML bool
+val no_everparse_h : unit -> ML bool
 
-val get_check_hashes : unit -> ML (option check_hashes_t)
+val check_hashes : unit -> ML (option check_hashes_t)
 
-val get_save_hashes : unit -> ML bool
+val save_hashes : unit -> ML bool
 
-val get_check_inplace_hashes : unit -> ML (list string)
+val check_inplace_hashes : unit -> ML (list string)
 
-val get_equate_types_list : unit -> ML (list (string & string))
+val equate_types_list : unit -> ML (list (string & string))
 
-val get_micro_step : unit -> ML (option micro_step_t)
+val micro_step : unit -> ML (option micro_step_t)
 
-val get_produce_c_from_existing_krml : unit -> ML bool
+val produce_c_from_existing_krml : unit -> ML bool
 
-val get_skip_deps : unit -> ML bool
+val skip_deps : unit -> ML bool
 
-val get_makefile : unit -> ML (option makefile_type)
+val makefile : unit -> ML (option makefile_type)
 
-val get_makefile_name : unit -> ML string
+val makefile_name : unit -> ML string
 
-val get_skip_o_rules : unit -> ML bool
+val skip_o_rules : unit -> ML bool
 
-val get_json : unit -> ML bool
+val json : unit -> ML bool
 
-val get_input_stream_binding : unit -> ML input_stream_binding_t
+val input_stream_binding : unit -> ML input_stream_binding_t
 
-val get_emit_output_types_defs : unit -> ML bool
+val emit_output_types_defs : unit -> ML bool
 
-val get_config_file : unit -> ML (option string)
+val config_file : unit -> ML (option string)
 
-val get_add_include : unit -> ML (list string)
+val add_include : unit -> ML (list string)
 
 val make_includes : unit -> ML string
 
 val config_module_name : unit -> ML (option string)
 
-val get_emit_smt_encoding: unit -> ML bool
+val emit_smt_encoding: unit -> ML bool
 
-val get_z3_test: unit -> ML (option string)
+val z3_test: unit -> ML (option string)
 
-val get_z3_pos_test: unit -> ML bool
+val z3_pos_test: unit -> ML bool
 
-val get_z3_neg_test: unit -> ML bool
+val z3_neg_test: unit -> ML bool
 
-val get_z3_witnesses: unit -> ML pos
+val z3_witnesses: unit -> ML pos
 
-val get_debug: unit -> ML bool
+val debug: unit -> ML bool
 
-val get_z3_diff_test: unit -> ML (option (string & string))
+val z3_diff_test: unit -> ML (option (string & string))
 
-val get_save_z3_transcript: unit -> ML (option string)
+val save_z3_transcript: unit -> ML (option string)
 
-val get_test_checker: unit -> ML (option string)
+val test_checker: unit -> ML (option string)
 
-val get_z3_branch_depth: unit -> ML nat
+val z3_branch_depth: unit -> ML nat
